Mise à jour de la contribution lc avec les fichiers envoyés par l'auteur
git-svn-id: svn://scm.gforge.inria.fr/svnroot/coq-contribs/branches/v8.1@836 0cf17b13-060f-0410-b1b1-c666bec9822a

Lc.v
@@ -11,16 +11,18 @@ Opaque app1.
 
 Section Lc.
 
+Implicit Type X Y Z : Set.
+
 Let r X : Eqv (term X) :=
   Build_Eqv (@lcr X) (@lcr_rfl X) (@lcr_sym X) (@lcr_trs X).
 Implicit Arguments r [X].
 
-Definition lc (X : Set) : Set := term X // r.
+Definition lc : Set -> Set := fun X => term X // r.
 
-Definition lc_class (X : Set) : term X -> lc X := class r.
+Definition lc_class X : term X -> lc X := class r.
 Notation "/ x" := (lc_class x).
 
-Lemma lc_class_eq : forall (X : Set) (x y : term X),
+Lemma lc_class_eq : forall X (x y : term X),
   x == y -> /x = /y.
 Proof.
 unfold lc_class. intros.
@@ -28,7 +30,7 @@ apply class_eq with (r := @r X). assumption.
 Qed.
 Hint Resolve lc_class_eq.
 
-Lemma lc_class_rel : forall (X : Set) (x y : term X),
+Lemma lc_class_rel : forall X (x y : term X),
   /x = /y -> x == y.
 Proof.
 unfold lc_class; simpl. intros.
@@ -36,18 +38,20 @@ apply class_rel with (r := @r X). assumption.
 Qed.
 Hint Resolve lc_class_rel.
 
-Lemma lc_class_surj : forall (X : Set) (u : lc X),
+Lemma lc_class_surj : forall X (u : lc X),
   exists a, /a = u.
 Proof.
-unfold r; simpl. intros. class u v. split with v. reflexivity.
+unfold r; simpl. intro X.
+apply (class_ind (fun u => exists a : term X, / a = u)).
+intros. split with x. reflexivity.
 Qed.
 Hint Resolve lc_class_surj.
 
-Definition lc_factor (X Y : Set) (f : term X -> Y)
+Definition lc_factor X Y (f : term X -> Y)
   (Hf : forall x y, x == y -> f x = f y) : lc X -> Y :=
   factor r f Hf.
 
-Lemma lc_factorize : forall (X Y : Set) (f : term X -> Y)
+Lemma lc_factorize : forall X Y (f : term X -> Y)
   (H : forall x y, x == y -> f x = f y),
     forall x,  lc_factor f H (/x) = f x.
 Proof.
@@ -55,11 +59,21 @@ unfold lc_factor, lc_class; simpl; intros. apply factorize.
 Qed.
 Hint Resolve lc_factorize.
 
-Definition lc_factor1 (X Y : Set) (f : term X -> term Y)
+Lemma lc_factor_cong : forall X Y (f g : term X -> Y) (x : lc X)
+  (Hf : forall x y, x == y -> f x = f y)
+  (Hg : forall x y, x == y -> g x = g y)
+  (H : forall x, f x = g x),
+  lc_factor f Hf x = lc_factor g Hg x.
+Proof.
+intros. unfold lc_factor.
+apply factor_extens. assumption.
+Qed.
+
+Definition lc_factor1 X Y (f : term X -> term Y)
   (Hf : forall x y, x == y -> f x == f y) : lc X -> lc Y :=
   factor1 r r f Hf.
 
-Lemma lc_factorize1 : forall (X Y : Set) (f : term X -> term Y)
+Lemma lc_factorize1 : forall X Y (f : term X -> term Y)
   (H : forall x y, x == y -> f x == f y),
     forall x,  lc_factor1 f H (/x) = /f x.
 Proof.
@@ -67,14 +81,12 @@ unfold lc, lc_factor1, lc_class; simpl; intros. apply factorize1.
 Qed.
 Hint Resolve lc_factorize1.
 
-Definition lc_factor2 (X Y Z : Set)
-  (f : term X -> term Y -> term Z)
+Definition lc_factor2 X Y Z (f : term X -> term Y -> term Z)
   (Hf : forall x y z w, x == y -> z == w -> f x z == f y w) :
     lc X -> lc Y -> lc Z :=
   factor2 r r r f Hf.
 
-Lemma lc_factorize2 : forall (X Y Z : Set)
-  (f : term X -> term Y -> term Z)
+Lemma lc_factorize2 : forall X Y Z (f : term X -> term Y -> term Z)
   (H : forall x y z w, x == y -> z == w -> f x z == f y w),
     forall x y,  lc_factor2 f H (/x) (/y) = /f x y.
 Proof.
@@ -82,7 +94,7 @@ unfold lc, lc_factor2, lc_class; simpl; intros. apply factorize2.
 Qed.
 Hint Resolve lc_factorize2.
 
-Lemma lc_fun_lift : forall (X Y : Set) (f : X -> lc Y),
+Lemma lc_fun_lift : forall X Y (f : X -> lc Y),
   exists g : X -> term Y, f = fun x => /g x.
 Proof.
 intros. lift_fun f f'. exists f'. reflexivity.
@@ -90,10 +102,10 @@ Qed.
 
 Opaque lc lc_class lc_factor lc_factor1 lc_factor2.
 
-Definition lc_abs (X : Set) : lc (option X) -> lc X :=
+Definition lc_abs X : lc (option X) -> lc X :=
   lc_factor1 (@abs X) (@lcr_abs X).
 
-Lemma lc_abs_factorize : forall (X : Set) (x : term (option X)),
+Lemma lc_abs_factorize : forall X (x : term (option X)),
   lc_abs (/x) = / abs x.
 Proof.
 unfold lc_abs. intros. apply lc_factorize1.
@@ -101,10 +113,10 @@ Qed.
 
 Opaque lc_abs.
 
-Definition lc_app1 (X : Set) : lc X -> lc (option X) :=
+Definition lc_app1 X : lc X -> lc (option X) :=
   lc_factor1 (@app1 X) (@lcr_app1 X).
 
-Lemma lc_app1_factorize : forall (X : Set) (x : term X),
+Lemma lc_app1_factorize : forall X (x : term X),
   lc_app1 (/x) = / app1 x.
 Proof.
 unfold lc_app1. intros. apply lc_factorize1.
@@ -112,10 +124,10 @@ Qed.
 
 Opaque lc_app1.
 
-Definition lc_app (X : Set) : lc X -> lc X -> lc X :=
+Definition lc_app X : lc X -> lc X -> lc X :=
   lc_factor2 (@app X) (@lcr_app X).
 
-Lemma lc_app_factorize : forall (X : Set) (x y : term X),
+Lemma lc_app_factorize : forall X (x y : term X),
   lc_app (/x) (/y) = / app x y.
 Proof.
 unfold lc_app. intros. apply lc_factorize2.
@@ -123,14 +135,13 @@ Qed.
 
 Opaque lc_app.
 
-Definition lc_var (X : Set) (x : X) : lc X := / var x.
+Definition lc_var X (x : X) : lc X := / var x.
 
 
-Definition lc_fct (X Y : Set) (f : X -> Y) : lc X -> lc Y :=
+Definition lc_fct X Y (f : X -> Y) : lc X -> lc Y :=
   lc_factor1 (fct f) (lcr_fct f).
 
-Lemma lc_fct_factorize : forall (X Y : Set)
-  (f : X -> Y) (x : term X),
+Lemma lc_fct_factorize : forall X Y (f : X -> Y) (x : term X),
   lc_fct f (/x) = /fct f x.
 Proof.
 unfold lc_fct; intros. apply lc_factorize1.
@@ -138,24 +149,29 @@ Qed.
 
 Opaque lc_fct.
 
-Definition lc_comm (X Y : Set)
-  (f : X -> lc Y) (x : option X) : lc (option Y) :=
+Definition lc_comm X Y (f : X -> lc Y) (x : option X) : lc (option Y) :=
   match x with
   | Some a => lc_fct (@Some Y) (f a)
   | None => lc_var None
   end.
 
-Fixpoint lc_subst_fix (X Y : Set) (f : X -> lc Y)
-  (x : term X) { struct x } : lc Y :=
+Fixpoint lc_bind_fix X Y (f : X -> lc Y) (x : term X) { struct x } : lc Y :=
   match x with
   | var x => f x
-  | app x y => lc_app (lc_subst_fix f x) (lc_subst_fix f y)
-  | abs x => lc_abs (lc_subst_fix (lc_comm f) x)
+  | app x y => lc_app (lc_bind_fix f x) (lc_bind_fix f y)
+  | abs x => lc_abs (lc_bind_fix (lc_comm f) x)
   end.
 
-Remark lc_subst_fix_factorize : forall (X Y : Set)
-  (f : X -> term Y) (x : term X),
-  lc_subst_fix (fun a => /f a) x = /(x //= f).
+Lemma lc_bind_fix_fun_cong : forall X (x : term X) Y (f g : X -> lc Y),
+  (forall u, f u = g u) -> lc_bind_fix f x = lc_bind_fix g x.
+Proof.
+induction x; simpl; intros; auto.
+f_equal. apply IHx.
+destruct u; simpl; auto.
+Qed.
+
+Remark lc_bind_fix_factorize : forall X Y (f : X -> term Y) (x : term X),
+  lc_bind_fix (fun a => /f a) x = /(x //= f).
 Proof.
 intros.
 generalize Y f; clear Y f.
@@ -164,116 +180,121 @@ reflexivity.
 rewrite IHx1.
 rewrite IHx2.
 apply lc_app_factorize.
-rewrite <- lc_abs_factorize.
-congr.
+rewrite <- lc_abs_factorize. f_equal.
 rewrite <- IHx.
-congr.
-extens u.
+apply lc_bind_fix_fun_cong.
 destruct u; simpl.
-rewrite lc_fct_factorize.
-reflexivity.
+rewrite lc_fct_factorize. reflexivity.
 reflexivity.
 Qed.
 
-Remark lc_subst_fix_wd : forall (X Y : Set)
-  (f : X -> lc Y) (x y : term X),
-  x == y -> lc_subst_fix f x = lc_subst_fix f y.
+Remark lc_bind_fix_wd : forall X Y (f : X -> lc Y) (x y : term X),
+  x == y -> lc_bind_fix f x = lc_bind_fix f y.
 Proof.
 intros. destruct (lc_fun_lift f) as (f', Hf). subst f.
-do 2 rewrite lc_subst_fix_factorize. apply lc_class_eq.
-apply lcr_subst. intros. apply lcr_rfl. assumption.
+do 2 rewrite lc_bind_fix_factorize. apply lc_class_eq.
+apply lcr_bind. intros. apply lcr_rfl. assumption.
 Qed.
 
-Definition lc_subst (X Y : Set) (f : X -> lc Y) : lc X -> lc Y :=
-  lc_factor (lc_subst_fix f) (lc_subst_fix_wd f).
+Definition lc_bind X Y (f : X -> lc Y) : lc X -> lc Y :=
+  lc_factor (lc_bind_fix f) (lc_bind_fix_wd f).
 
-Lemma lc_subst_factorize : forall (X Y : Set)
-  (f : X -> term Y) (x : term X),
-  lc_subst (fun a => /f a) (/x) = /(x //= f).
+Lemma lc_bind_factorize : forall X Y (f : X -> term Y) (x : term X),
+  lc_bind (fun a => /f a) (/x) = /(x //= f).
 Proof.
-unfold lc_subst. intros.
-rewrite lc_factorize. apply lc_subst_fix_factorize.
+unfold lc_bind. intros.
+rewrite lc_factorize. apply lc_bind_fix_factorize.
 Qed.
 
-Opaque lc_subst.
-
-Lemma lc_fct_as_subst : forall (X Y : Set) (f : X -> Y),
-  lc_fct f = lc_subst (fun a => lc_var (f a)).
+Lemma lc_bind_fun_cong : forall X Y (f g : X -> lc Y) (x : lc X),
+  (forall u, f u = g u) -> lc_bind f x = lc_bind g x.
 Proof.
-unfold lc_var. intros. extens.
+intros.
+unfold lc_bind.
+apply lc_factor_cong.
+intros.
+apply lc_bind_fix_fun_cong.
+assumption.
+Qed.
+
+Opaque lc_bind.
+
+Lemma lc_fct_as_bind : forall X Y (f : X -> Y) (x : lc X),
+  lc_fct f x = lc_bind (fun a => lc_var (f a)) x.
+Proof.
+unfold lc_var. intros.
 destruct (lc_class_surj x) as [y Hy]. subst x.
-rewrite lc_fct_factorize. rewrite fct_as_subst.
-rewrite <- lc_subst_factorize. reflexivity.
+rewrite lc_fct_factorize. rewrite slc_fct_as_bind.
+rewrite <- lc_bind_factorize. reflexivity.
 Qed.
 
-Lemma lc_subst_assoc : forall (X Y Z : Set)
-  (f : X -> lc Y) (g : Y -> lc Z) (x : lc X),
-  lc_subst g (lc_subst f x) =
-    lc_subst (fun a => lc_subst g (f a)) x.
+Lemma lc_bind_assoc :
+  forall X Y Z (f : X -> lc Y) (g : Y -> lc Z) (x : lc X),
+  lc_bind g (lc_bind f x) = lc_bind (fun a => lc_bind g (f a)) x.
 Proof.
 intros.
 destruct (lc_class_surj x) as (y, Hy). subst x.
 destruct (lc_fun_lift f) as (f', Hf). subst f.
-rewrite lc_subst_factorize.
+rewrite lc_bind_factorize.
 destruct (lc_fun_lift g) as (g', Hg). subst g.
-rewrite lc_subst_factorize.
-rewrite subst_subst.
-rewrite <- lc_subst_factorize.
-congr. extens. rewrite lc_subst_factorize. reflexivity.
+rewrite lc_bind_factorize.
+rewrite slc_bind_bind.
+rewrite <- lc_bind_factorize.
+apply lc_bind_fun_cong. intros.
+rewrite lc_bind_factorize. reflexivity.
 Qed.
 
-Lemma lc_subst_var : forall (X Y : Set) (f : X -> lc Y) (x : X),
-  lc_subst f (lc_var x) = f x.
+Lemma lc_bind_var : forall X Y (f : X -> lc Y) (x : X),
+  lc_bind f (lc_var x) = f x.
 Proof.
 unfold lc_var. intros.
 destruct (lc_fun_lift f) as (f', Hf). subst f.
-rewrite lc_subst_factorize. rewrite subst_var. reflexivity.
+rewrite lc_bind_factorize. rewrite slc_bind_var. reflexivity.
 Qed.
 
-Lemma lc_var_subst : forall (X : Set) (x : lc X),
-  lc_subst (@lc_var X) x = x.
+Lemma lc_var_bind : forall X (x : lc X),
+  lc_bind (@lc_var X) x = x.
 Proof.
 unfold lc_var. intros.
 destruct (lc_class_surj x) as (y, Hy). subst x.
-rewrite lc_subst_factorize.
-rewrite var_subst. reflexivity.
+rewrite lc_bind_factorize.
+rewrite slc_var_bind. reflexivity.
 Qed.
 
-Lemma lc_subst_abs : forall (X Y : Set)
-  (f : X -> lc Y) (x : lc (option X)),
-  lc_subst f (lc_abs x) = lc_abs (lc_subst (lc_comm f) x).
+Lemma lc_bind_abs : forall X Y (f : X -> lc Y) (x : lc (option X)),
+  lc_bind f (lc_abs x) = lc_abs (lc_bind (lc_comm f) x).
 Proof.
 intros.
 destruct (lc_class_surj x) as (y, Hy). subst x.
 rewrite lc_abs_factorize.
 destruct (lc_fun_lift f) as (f', Hf). subst f.
-rewrite lc_subst_factorize. simpl.
-rewrite <- lc_abs_factorize. congr.
-rewrite <- lc_subst_factorize. congr.
-extens. destruct x; simpl. 2:reflexivity.
+rewrite lc_bind_factorize. simpl.
+rewrite <- lc_abs_factorize. f_equal.
+rewrite <- lc_bind_factorize.
+apply lc_bind_fun_cong. intro.
+destruct u; simpl. 2:reflexivity.
 rewrite lc_fct_factorize. reflexivity.
 Qed.
 
-Lemma lc_subst_app1 : forall (X Y : Set)
-  (f : X -> lc Y) (x : lc X),
-  lc_subst (lc_comm f) (lc_app1 x) = lc_app1 (lc_subst f x).
+Lemma lc_bind_app1 : forall X Y (f : X -> lc Y) (x : lc X),
+  lc_bind (lc_comm f) (lc_app1 x) = lc_app1 (lc_bind f x).
 Proof.
 intros.
 destruct (lc_class_surj x) as (y, Hy). subst x.
 destruct (lc_fun_lift f) as (f', Hf). subst f.
 rewrite lc_app1_factorize.
-rewrite lc_subst_factorize.
+rewrite lc_bind_factorize.
 rewrite lc_app1_factorize.
-replace (lc_comm (fun x : X => / f' x))
-  with (fun a => /comm f' a).
-rewrite lc_subst_factorize.
-rewrite subst_app1. rewrite app1_app.
-unfold shift. rewrite fct_subst. reflexivity.
-extens a; destruct a; simpl. 2:reflexivity.
+transitivity (lc_bind (fun a => /comm f' a) (/ app1 y)).
+apply lc_bind_fun_cong.
+destruct u; simpl. 2:reflexivity.
 rewrite lc_fct_factorize. reflexivity.
+rewrite lc_bind_factorize.
+rewrite slc_bind_app1. rewrite app1_app.
+unfold shift. rewrite slc_fct_bind. reflexivity.
 Qed.
 
-Lemma lc_eta : forall (X : Set) (x : lc X),
+Lemma lc_eta : forall X (x : lc X),
   lc_abs (lc_app1 x) = x.
 Proof.
 intros.
@@ -282,15 +303,15 @@ rewrite lc_app1_factorize. rewrite lc_abs_factorize.
 apply lc_class_eq. apply lcr_eta.
 Qed.
 
-Lemma lc_beta : forall (X : Set) (x : lc (option X)),
+Lemma lc_beta : forall X (x : lc (option X)),
   lc_app1 (lc_abs x) = x.
 intros.
 destruct (lc_class_surj x) as (y, Hy). subst x.
 rewrite lc_abs_factorize. rewrite lc_app1_factorize.
 apply lc_class_eq. apply lcr_beta. 
 rewrite app1_app. unfold shift. simpl.
-apply beta_intro2. rewrite subst_fct.
-apply var_subst_match.
+apply beta_intro_alt. rewrite slc_bind_fct.
+apply slc_var_bind_match.
 destruct u; reflexivity.
 Qed.
 
